Add interpretation for !τ.

theories/examples/ill.v
@@ -1,4 +1,5 @@
 From stdpp Require Import gmap fin_maps fin_sets stringmap.
+From iris.base_logic.lib Require Import invariants.
 From actris.channel Require Import proofmode.
 From actris.utils Require Import syntax_facts.
 
@@ -106,7 +107,7 @@ Context `{!heapG Σ, !chanG Σ}.
 
 Program Definition iProto_server_aux
     (P : iProto Σ) : iProto Σ -n> iProto Σ := λne self,
-   (<? c> MSG c {{ ▷ c ↣ iProto_dual P }}; self)%proto.
+   (<? c> MSG c {{ c ↣ P }}; self)%proto.
 Next Obligation. solve_proper. Qed.
 
 Instance iProto_server_contractive P :
@@ -115,7 +116,7 @@ Proof. solve_contractive. Qed.
 
 Definition iProto_server (P : iProto Σ) := fixpoint (iProto_server_aux P).
 Lemma iProto_server_unfold P :
-  (iProto_server P ≡ <? c> MSG c {{ ▷ c ↣ iProto_dual P }}; iProto_server P)%proto.
+  (iProto_server P ≡ <? c> MSG c {{ c ↣ P }}; iProto_server P)%proto.
 Proof.
   rewrite /iProto_server. eapply (fixpoint_unfold (iProto_server_aux P)).
 Qed.
@@ -133,15 +134,20 @@ Fixpoint interp_ty (τ : ty) : iProto Σ :=
 
 Arguments interp_ty τ%ty.
 
-Definition tyctx := gmap string ty.
-Definition interp_seq (Δ : tyctx) (e : expr) (x : string) (τ : ty) : iProp Σ :=
-  ∀ (cs : gmap string val) (* substitution map *)
-    (o : val),    (* "output" channel *)
-    ([∗ map] x ↦ σ;c ∈ Δ;cs, c ↣ iProto_dual (interp_ty σ)) -∗
-  o ↣ interp_ty τ -∗
-  WP (subst_map (<[x:=o]>cs) e) {{ _, o ↣ END (* ∗ ([∗ map] x ↦ σ;c ∈ Δ;cs, c ↣ END) *) }}%I.
+Definition nctx (u : val) := nroot.@"illctx".@u.
 
-Notation "Δ '⊢ₗ' P ':' '(' c ':' τ ')'" := (interp_seq Δ%ty P c τ%ty) (at level 74, P, c, τ at next level).
+Definition tyctx := gmap string ty.
+Definition interp_seq (Γ : tyctx) (Δ : tyctx) (e : expr) (x : string) (τ : ty) : iProp Σ :=
+  □
+  ∀ (ss cs : gmap string val) (* substitution maps *)
+    (o : val),    (* "output" channel *)
+  ⌜ss ##ₘ cs⌝ -∗
+  ([∗ map] x ↦ σ;u ∈ Γ;ss, inv (nctx u) (u ↣ iProto_dual (iProto_server (interp_ty σ)))) -∗
+  ([∗ map] x ↦ σ;c ∈ Δ;cs, c ↣ iProto_dual (interp_ty σ)) -∗
+  o ↣ interp_ty τ -∗
+  WP (subst_map (<[x:=o]>(ss ∪ cs)) e) {{ _, o ↣ END }}%I.
+
+Notation "Γ '&;' Δ '⊢ₗ' P ':' '(' c ':' τ ')'" := (interp_seq Γ%ty Δ%ty P%E c τ%ty) (at level 74, P, c, τ at next level).
 
 (* Attempt to prove that [cs2 !! y = None] *)
 Ltac assert_not_in_map cs2 y :=
@@ -169,119 +175,381 @@ Ltac assert_in_map cs y :=
   let yv := fresh "y" in let Hyv := fresh "Hy" in
   assert_in_map_ cs y yv Hyv.
 
-Lemma cut_ Δ1 Δ2 (x y : string) τ1 τ2 e1 e2 :
+
+
+
+Lemma cut_ Γ Δ1 Δ2 (x y : string) τ1 τ2 e1 e2 :
   x ≠ y →
   Δ1 !! y = None →
   Δ2 !! y = None →
+  Γ !! x = None →
+  Γ !! y = None →
   Δ1 ##ₘ Δ2 →
-  is_closed_expr_set ({[x]} ∪ dom _ Δ1) e1 →
-  is_closed_expr_set ({[x;y]} ∪ dom _ Δ2) e2 →
-  (Δ1 ⊢ₗ e1 : (x : τ1)) -∗
-  ((<[x:=τ1]>Δ2) ⊢ₗ e2 : (y : τ2)) -∗
-  (Δ1 ∪ Δ2 ⊢ₗ (let: x := start_chan (λ: x, e1) in e2) : (y : τ2)).
+  is_closed_expr_set ({[x]} ∪ dom _ Δ1 ∪ dom _ Γ) e1 →
+  is_closed_expr_set ({[x;y]} ∪ dom _ Δ2 ∪ dom _ Γ) e2 →
+  (Γ &; Δ1 ⊢ₗ e1 : (x : τ1)) -∗
+  (Γ &; (<[x:=τ1]>Δ2) ⊢ₗ e2 : (y : τ2)) -∗
+  (Γ &; Δ1 ∪ Δ2 ⊢ₗ (let: x := start_chan (λ: x, e1) in e2) : (y : τ2)).
 Proof.
-  intros Hxy Hy1 Hy2 HΔ Hclosed1 Hclosed2. iIntros "H1 H2".
-  iIntros (cs oy) "HΔ Hoy". simpl.
+  intros Hxy Hy1 Hy2 Hx0 Hy0 HΔ Hclosed1 Hclosed2. iIntros "#H1 #H2".
+  iModIntro. iIntros (ss cs oy Hsscs) "#HΓ HΔ Hoy". simpl.
   rewrite big_sepM2_union_l //.
   iDestruct "HΔ" as (cs1 cs2 Hcs ->) "[HΔ HΔ']".
   iAssert (⌜dom stringset Δ1 = dom stringset cs1⌝)%I as %Hdom1.
-  { by rewrite big_sepM2_dom. }
+  { by rewrite (big_sepM2_dom _ Δ1). }
   iAssert (⌜dom stringset Δ2 = dom stringset cs2⌝)%I as %Hdom2.
   { by rewrite (big_sepM2_dom _ Δ2). }
+  iAssert (⌜dom stringset Γ = dom stringset ss⌝)%I as %Hdom0.
+  { by rewrite (big_sepM2_dom _ Γ). }
 
   assert_not_in_map cs1 y.
   assert_not_in_map cs2 y.
+  assert_not_in_map ss x.
+  assert_not_in_map ss y.
 
+  eapply map_disjoint_union_r in Hsscs.
+  destruct Hsscs as [Hsscs1 Hsscs2].
   wp_smart_apply (start_chan_spec (iProto_dual (interp_ty τ1)) with "[H1 HΔ]").
   { iNext. iIntros (c) "Hc".
     rewrite iProto_dual_involutive. wp_pures.
-    iSpecialize ("H1" with "HΔ Hc").
+    iSpecialize ("H1" with "[%] HΓ HΔ Hc"); eauto.
     rewrite -subst_map_insert.
-    - assert (subst_map (<[x:=c]> cs1) e1
-              = subst_map (<[x:=c]> (<[y:=oy]> (cs1 ∪ cs2))) e1) as ->.
+    - assert (subst_map (<[x:=c]> (ss ∪ cs1)) e1
+              = subst_map (<[x:=c]> (<[y:=oy]> (ss ∪ (cs1 ∪ cs2)))) e1) as ->.
       { eapply subst_map_agree_weaken; eauto.
-        - by rewrite Hdom1 dom_insert_L.
+        - rewrite Hdom1 Hdom0 dom_insert_L. by set_solver.
         - eapply insert_mono.
-          rewrite insert_union_l. etrans; last eapply map_union_subseteq_l.
+          rewrite insert_union_l.
+          rewrite assoc_L.
+          etrans; last eapply map_union_subseteq_l.
+          eapply map_union_mono_r.
+          { eapply map_disjoint_insert_l. eauto. }
           eapply insert_subseteq.
-          eapply not_elem_of_dom. rewrite -Hdom1.
+          eapply not_elem_of_dom. rewrite -Hdom0.
           by eapply not_elem_of_dom. }
       iApply (wp_wand with "H1"). eauto. }
   iIntros (xc) "Hx". wp_pures.
-  iSpecialize ("H2" $! (<[x:=xc]>cs2) with "[HΔ' Hx] Hoy").
-  { iApply (big_sepM2_insert_2 with "[Hx]"); eauto. }
-  rewrite -subst_map_insert.
-  cut (subst_map (<[y:=oy]> (<[x:=xc]> cs2)) e2
-       = subst_map (<[x:=xc]> (<[y:=oy]> (cs1 ∪ cs2))) e2); first by intros ->.
-  rewrite insert_commute//.
-  eapply subst_map_fact_2; eauto.
-  by rewrite -Hdom2.
+  iSpecialize ("H2" $! ss (<[x:=xc]>cs2) with "[%] HΓ [HΔ' Hx] Hoy").
+  - eapply map_disjoint_insert_r. eauto.
+  - iApply (big_sepM2_insert_2 with "[Hx]"); eauto.
+  - rewrite -subst_map_insert.
+    rewrite -insert_union_r//.
+    rewrite insert_commute//.
+    cut (subst_map (<[x:=xc]> (<[y:=oy]> (ss ∪ cs2))) e2
+         = subst_map (<[x:=xc]> (<[y:=oy]> (ss ∪ (cs1 ∪ cs2)))) e2); first by intros ->.
+    rewrite assoc_L (map_union_comm ss cs1) // -assoc_L.
+    eapply subst_map_fact_2; eauto.
+    + rewrite dom_union_L -Hdom2 -Hdom0.
+      assert (({[x; y]} ∪ (dom stringset Γ ∪ dom stringset Δ2))
+                = ({[x; y]} ∪ dom stringset Δ2 ∪ dom stringset Γ)) as ->.
+      { set_unfold. tauto. }
+      done.
+    + eapply lookup_union_None; eauto.
+    + eapply map_disjoint_union_r; eauto.
 Qed.
 
-Lemma tone_right (x : string) :
-  (⊢ ∅ ⊢ₗ send (Var x) #() : (x : 1)).
+Lemma tcopy Γ Δ (x y u : string) τ1 τ2 e :
+  x ≠ y →
+  y ≠ u →
+  u ≠ "z" →
+  y ≠ "z" →
+  Δ !! x = None →
+  Γ !! x = None →
+  Γ !! u = Some τ1 →
+  is_closed_expr_set ({[x;y]} ∪ dom _ Δ ∪ dom _ Γ) e →
+  (Γ &; (<[x:=τ1]>Δ) ⊢ₗ e : (y : τ2)) -∗
+  (Γ &; Δ ⊢ₗ (let: x := start_chan (λ: "z", send u "z") in e) : (y : τ2)).
 Proof.
-  iIntros (vs o) "Hemp Ho". wp_pures.
-  rewrite big_sepM2_empty_r. iDestruct "Hemp" as "->".
+  intros Hxy Hyu Huz Hyz HΔ1 HΔ HG Hclosed1. iIntros "#H1".
+  iModIntro.
+  iIntros (ss cs oy Hsscs) "#HΓ HΔ Hoy".
+
+  iAssert (⌜dom stringset Δ = dom stringset cs⌝)%I as %Hdom.
+  { by rewrite (big_sepM2_dom _ Δ). }
+  iAssert (⌜dom stringset Γ = dom stringset ss⌝)%I as %Hdom0.
+  { by rewrite (big_sepM2_dom _ Γ). }
+  assert (u ∈ dom stringset Γ).
+  { eapply elem_of_dom. eauto. }
+
+  assert_not_in_map cs x.
+  assert_not_in_map ss x.
+  assert_in_map_ ss u uv Huv.
+
+  simpl. rewrite lookup_delete_ne//. rewrite lookup_delete.
+  rewrite lookup_insert_ne//.
+  rewrite (lookup_union_Some_l _ _ _ _ Huv).
+
+  wp_smart_apply (start_chan_spec (iProto_dual (interp_ty τ1)) with "[]").
+  { iNext. iIntros (c) "Hc". wp_pures.
+    rewrite iProto_dual_involutive.
+    iApply (send_spec_atomic val (λ v, v ↣ interp_ty τ1) True%I c id with "Hc [//]").
+    iModIntro. iAssert (inv (nctx uv) (uv ↣ iProto_dual (iProto_server (interp_ty τ1))))%I as "#Hinv".
+    {  rewrite (big_sepM2_insert_acc _ Γ ss u) //. by iDestruct "HΓ" as "[$ _]". }
+    iInv (nctx uv) as "Huv" "Hcl". iModIntro.
+    rewrite {2}iProto_server_unfold.
+    rewrite iProto_dual_message /=.
+    rewrite iMsg_dual_exist.
+    iExists (λ _, iProto_dual (iProto_server (interp_ty τ1))).
+    assert ((<! (x0 : val)> MSG x0 {{ x0 ↣ interp_ty τ1 }}; iProto_dual (iProto_server (interp_ty τ1)))%proto
+               ≡ (<! (x0 : val)> iMsg_dual (MSG x0 {{ x0 ↣ interp_ty τ1 }}; iProto_server (interp_ty τ1)))%proto) as ->.
+    { f_equiv. f_equiv. intros xx.
+      by rewrite iMsg_dual_base. }
+    iFrame "Huv". iSplit.
+    { iIntros "HH". iApply "Hcl".
+      rewrite {3}iProto_server_unfold.
+      rewrite iProto_dual_message /= iMsg_dual_exist. iFrame "HH". }
+    iIntros "[Huv _]". by iApply "Hcl". }
+  iIntros (xc) "Hx". wp_pures.
+  iSpecialize ("H1" $! ss (<[x:=xc]>cs) with "[%] HΓ [HΔ Hx] Hoy").
+  - eapply map_disjoint_insert_r. eauto.
+  - iApply (big_sepM2_insert_2 with "[Hx]"); eauto.
+  - rewrite -subst_map_insert.
+    rewrite insert_commute //.
+    rewrite -(insert_union_r _ _ x)//.
+Qed.
+
+
+Definition loop_ : val :=
+  (rec: "f" "z" "t" := let: "x" := recv "z" in Fork ("t" "x") ;; "f" "z" "t")%V.
+
+Lemma cut_bang Γ Δ (x y u : string) τ1 τ2 e1 e2 :
+  x ≠ y →
+  x ≠ u →
+  u ≠ y →
+  is_closed_expr_set ({[x]} ∪ dom stringset Γ) e1 →
+  is_closed_expr_set ({[u;y]} ∪ dom stringset Δ ∪ dom stringset Γ) e2 →
+  Δ !! x = None →
+  Δ !! u = None →
+  Γ !! x = None →
+  Γ !! y = None →
+  Γ !! u = None →
+  (Γ &; ∅ ⊢ₗ e1 : (x : τ1)) -∗
+  ((<[u:=τ1]>Γ) &; Δ ⊢ₗ e2 : (y : τ2)) -∗
+  Γ &; Δ ⊢ₗ (let: u := start_chan (λ: u, e2) in loop_ u (λ: x, e1)) : (y : τ2).
+Proof.
+  intros Hxy Hxu Huy He1 He2 Hx Hx2 Hy2 Hu Hu2. iIntros "#H1 #H2".
+  iModIntro. iIntros (ss cs oy Hsscs) "#HΓ HΔ Hoy".
+  iAssert (⌜dom stringset Δ = dom stringset cs⌝)%I as %Hdom1.
+  { by rewrite (big_sepM2_dom _ Δ). }
+  iAssert (⌜dom stringset Γ = dom stringset ss⌝)%I as %Hdom0.
+  { by rewrite (big_sepM2_dom _ Γ). }
+
+  assert_not_in_map cs x.
+  assert_not_in_map cs u.
+  assert_not_in_map ss x.
+  assert_not_in_map ss y.
+  assert_not_in_map ss u.
+
+  simpl.
+  rewrite lookup_delete.
+  wp_pures.
+
+  wp_smart_apply (start_chan_spec (iProto_server (interp_ty τ1)) with "[-]").
+  { iNext.
+    iIntros (uv) "Hu". wp_pures.
+    iMod (inv_alloc (nctx uv) _  (uv ↣ iProto_dual (iProto_server (interp_ty τ1))) with "[Hu]")  as "#Hinv".
+    { by iNext. }
+    iSpecialize ("H2" $! (<[u:=uv]> ss) cs oy with "[%]").
+    { eapply map_disjoint_insert_l_2; eauto. }
+    iSpecialize ("H2" with "[] HΔ Hoy").
+    - rewrite big_sepM2_insert //. iFrame "HΓ Hinv".
+    - rewrite -subst_map_insert. rewrite -insert_union_l.
+      rewrite insert_commute//.
+      iApply (wp_wand with "H2"). eauto. }
+  iIntros (c) "Hc". wp_pure _.
+  wp_pure _.
+  rewrite decide_left//.
+  case_decide; last naive_solver.
+  rewrite delete_commute//. rewrite -subst_map_insert.
+  rewrite delete_notin; last first.
+  { rewrite lookup_insert_ne//. eapply lookup_union_None. eauto. }
+  wp_pures.
+  iLöb as "IH". wp_rec. wp_pures.
+  rewrite {2}iProto_server_unfold. wp_recv (xv) as "Hx". wp_pures.
+  wp_bind (Fork _). iApply (wp_fork with "[Hx]").
+  { iApply (wp_wand _ _ _ (λ _, xv ↣ END)%proto with "[Hx]").
+    { iSpecialize ("H1" $! ss ∅ xv with "[%] HΓ [] Hx").
+      - eapply map_disjoint_empty_r.
+      - by iApply big_sepM2_empty.
+      - rewrite subst_map_insert. rewrite right_id.
+        rewrite -subst_map_insert.
+        wp_rec.
+        rewrite -(delete_notin (<[u:=c]> _) x); last first.
+        {  rewrite !lookup_insert_ne//.
+           eapply lookup_union_None; eauto. }
+        rewrite -subst_map_insert.
+        assert (subst_map (<[x:=xv]> ss) e1 = subst_map (<[x:=xv]> (<[u:=c]> (<[y:=oy]> (ss ∪ cs)))) e1) as ->.
+        { eapply subst_map_agree_weaken; eauto.
+          - by rewrite dom_insert_L Hdom0.
+          - eapply insert_mono. do 2 eapply insert_subseteq_r=>//.
+            eapply map_union_subseteq_l. }
+        iApply "H1". }
+      iNext. iIntros (?) "_". done. }
+  iNext. wp_pure _. wp_pure _. by iApply "IH".
+Qed.
+
+Lemma tofc_right Γ e (x y : string) τ :
+  x ≠ y →
+  Γ !! x = None →
+  is_closed_expr_set ({[y]} ∪ dom stringset Γ) e →
+  (Γ &; ∅ ⊢ₗ e : (y : τ)) -∗
+  (Γ &; ∅ ⊢ₗ (loop_ x (λ: y, e)) : (x : ! τ)).
+Proof.
+  intros Hxy Hx0 He. iIntros "#H".
+  iModIntro. iIntros (ss cs o Hsscs) "#Hss Hemp Ho". simpl.
+
+  rewrite lookup_insert.
+
+  iAssert (⌜dom stringset Γ = dom stringset ss⌝)%I as %Hdom0.
+  { by rewrite (big_sepM2_dom _ Γ). }
+  iAssert (⌜dom stringset ∅ = dom stringset cs⌝)%I as %Hdom1.
+  { by rewrite (big_sepM2_dom _ _ cs). }
+  assert (cs = ∅) as ->.
+  { eapply dom_empty_inv_L. simpl in Hdom1.
+    by rewrite -Hdom1 dom_empty_L. }
+  assert_not_in_map ss x.
+
+  iClear "Hemp". wp_pures.
+  iLöb as "IH". wp_rec. wp_pures.
+  rewrite {2}iProto_server_unfold.
+  wp_recv (yv) as "Hy". wp_pures.
+  rewrite right_id.
+  wp_bind (Fork _). iApply (wp_fork with "[Hy]").
+  { iNext. wp_rec. rewrite -subst_map_insert.
+    iSpecialize ("H" $! ss ∅ yv with "[%] Hss [] Hy").
+    { eapply map_disjoint_empty_r. }
+    { by iApply big_sepM2_empty. }
+    rewrite right_id.
+    rewrite (subst_map_agree_weaken e ({[y]} ∪ dom stringset Γ) (<[y:=yv]> ss) (<[y:=yv]> (<[x:=o]> ss)))//. 
+    2:{ by rewrite dom_insert_L Hdom0. }
+    2:{ eapply insert_mono. eapply insert_subseteq_r; eauto. }
+    iApply (wp_wand with "H"). eauto. }
+  iNext. wp_pures. by iApply "IH".
+Qed.
+
+Lemma tofc_left Γ Δ e (x y : string) τ σ :
+  x ≠ y →
+  Γ !! y = None →
+  Δ !! y = None →
+  is_closed_expr_set ({[x;y]} ∪ dom _ Δ ∪ dom _ Γ) e →
+  (<[y:=τ]>Γ &; Δ ⊢ₗ e : (x : σ)) -∗
+  (Γ &; (<[y:=tofc τ]>Δ) ⊢ₗ e : (x : σ)).
+Proof.
+  intros Hxy Hy0 Hy1 He. iIntros "#H".
+  iModIntro. iIntros (ss cs xv Hsscs) "Hss Hcs Hx".
+  iAssert (⌜dom stringset (<[y:=(tofc τ)]>Δ) = dom stringset cs⌝)%I as %Hdom1.
+  { by rewrite (big_sepM2_dom _ (<[y:=(tofc τ)]>Δ)). }
+  iAssert (⌜dom stringset Γ = dom stringset ss⌝)%I as %Hdom0.
+  { by rewrite (big_sepM2_dom _ Γ). }
+
+  assert_in_map_ cs y yv Hyv.
+  assert_not_in_map ss y.
+
+  assert (cs = <[y:=yv]>(delete y cs)) as Hcs.
+  { rewrite insert_delete insert_id//. }
+  rewrite {1}Hcs.
+  rewrite big_sepM2_insert//; last first.
+  { eapply lookup_delete. }
+  iDestruct "Hcs" as "[Hy Hcs]".
+  iSimpl in "Hy".
+  iMod (inv_alloc (nctx yv) _  (yv ↣ iProto_dual (iProto_server (interp_ty τ))) with "[Hy]")  as "#Hinv".
+  { by iNext. }
+  iSpecialize ("H" $! (<[y:=yv]>ss) (delete y cs) with "[%] [Hss] Hcs Hx").
+  { eapply map_disjoint_insert_l. split.
+    + eapply lookup_delete.
+    + by eapply map_disjoint_delete_r. }
+  iApply (big_sepM2_insert_2 with "[] Hss").
+  { simpl. by iFrame. }
+  rewrite -insert_union_l.
+  rewrite (insert_union_r ss _ y)//.
+  by rewrite -Hcs.
+Qed.
+
+Lemma tone_right Γ  (x : string) :
+  (⊢ Γ &; ∅ ⊢ₗ send (Var x) #() : (x : 1)).
+Proof.
+  iModIntro. iIntros (ss cs o Hsscs) "Hserv Hemp Ho". wp_pures.
   rewrite lookup_insert /=.
   wp_send with "[]"; eauto with iFrame.
 Qed.
 
-Lemma tone_left (x y : string) e Δ τ  :
+Lemma tone_left (x y : string) e Γ Δ τ  :
   x ≠ y →
   Δ !! y = None →
-  is_closed_expr_set ({[x]} ∪ dom _ Δ) e →
-  (Δ ⊢ₗ e : (x : τ)) -∗
-  (<[y:=1]>Δ) ⊢ₗ (recv y;; e) : (x : τ).
+  is_closed_expr_set ({[x]} ∪ dom _ Δ ∪ dom _ Γ) e →
+  (Γ &; Δ ⊢ₗ e : (x : τ)) -∗
+  (Γ &; (<[y:=1]>Δ) ⊢ₗ (recv y;; e) : (x : τ)).
 Proof.
-  iIntros (Hxy HΔ Hdome) "IH".
-  iIntros (cs o) "Hcs Ho". simpl.
+  iIntros (Hxy HΔ Hdome) "#IH".
+  iModIntro. iIntros (ss cs o Hsscs) "Hss Hcs Ho". simpl.
   rewrite lookup_insert_ne//.
   iAssert (⌜dom stringset (<[y:=1%ty]>Δ) = dom stringset cs⌝)%I as %Hdom1.
-  { by rewrite big_sepM2_dom. }
+  { by rewrite (big_sepM2_dom _ (<[y:=1%ty]>Δ)). }
+  iAssert (⌜dom stringset Γ = dom stringset ss⌝)%I as %Hdom0.
+  { by rewrite (big_sepM2_dom _ Γ). }
 
   assert_in_map_ cs y cy Hcy.
+  assert_not_in_map ss y.
+  { rewrite Hdom0. eapply not_elem_of_dom.
+    by eapply map_disjoint_Some_r. }
 
-  assert (cs = <[y:=cy]>(delete y cs)) as ->.
+  assert (cs = <[y:=cy]>(delete y cs)) as Hcs.
   { by rewrite insert_delete insert_id//. }
+  rewrite {1}Hcs.
   rewrite big_sepM2_insert; eauto; last first.
   { eapply lookup_delete. }
   iDestruct "Hcs" as "[Hx Hcs]". iSimpl in "Hx".
-  rewrite lookup_insert.
+  rewrite (lookup_union_Some_r _ _ _ _ Hsscs Hcy).
   wp_recv as "_". wp_pures.
-  iSpecialize ("IH" $! (delete y cs) with "Hcs Ho").
-  cut (subst_map (<[x:=o]> (delete y cs)) e
-       = subst_map (<[x:=o]> (<[y:=cy]> (delete y cs))) e); first by intros ->.
+  iSpecialize ("IH" $! ss (delete y cs) with "[%] Hss Hcs Ho").
+  { by apply map_disjoint_delete_r. }
+  cut (subst_map (<[x:=o]> (ss ∪ delete y cs)) e
+       = subst_map (<[x:=o]> (ss ∪ cs)) e); first by intros ->.
   eapply subst_map_agree_weaken; eauto.
-  { assert (y ∉ dom stringset Δ).
-    { by eapply not_elem_of_dom. }
-    set_unfold. naive_solver. }
-  eapply insert_mono. eapply insert_subseteq.
-  eapply lookup_delete.
+  { rewrite dom_insert_L dom_union_L (comm_L _ (dom stringset ss)) assoc_L.
+    repeat f_equiv; eauto.
+    rewrite dom_delete_L -Hdom1 dom_insert_L.
+    rewrite difference_union_distr_l_L.
+    rewrite difference_diag_L left_id_L.
+    rewrite -dom_delete_L.
+    rewrite delete_notin //. }
+  eapply insert_mono. eapply map_union_mono_l.
+  eapply delete_subseteq.
 Qed.
 
-Lemma tlolli_right (Δ : tyctx) τ1 τ2 e (x y : string) :
+Lemma tlolli_right (Γ Δ : tyctx) τ1 τ2 e (x y : string) :
   x ≠ y →
   Δ !! x = None →
   Δ !! y = None →
-  ((<[x:=τ1]>Δ) ⊢ₗ e : (y : τ2)) -∗
-  Δ ⊢ₗ (let: x := recv y in e) : (y : τ1 ⊸ τ2).
+  Γ !! x = None →
+  (Γ &; (<[x:=τ1]>Δ) ⊢ₗ e : (y : τ2)) -∗
+  Γ &; Δ ⊢ₗ (let: x := recv y in e) : (y : τ1 ⊸ τ2).
 Proof.
-  intros Hxy Hx Hy. iIntros "H".
-  iIntros (cs oy) "HΔ Hoy". wp_pures.
-  rewrite lookup_insert.
+  intros Hxy Hx Hy Hx'. iIntros "#H". iModIntro.
+  iIntros (ss cs oy Hsscs) "HΓ HΔ Hoy".
+
+  iAssert (⌜dom stringset Γ = dom stringset ss⌝)%I as %Hdom0.
+  { by rewrite (big_sepM2_dom _ Γ). }
+  assert_not_in_map ss x.
+
+  wp_pures. rewrite lookup_insert.
   iSimpl in "Hoy".
   wp_recv (cx) as "Hx". wp_pures.
   rewrite -subst_map_insert.
-  iSpecialize ("H" $! (<[x:=cx]>cs) with "[Hx HΔ] Hoy").
+  iSpecialize ("H" $! ss (<[x:=cx]>cs) with "[%] HΓ [Hx HΔ] Hoy").
+  { by eapply map_disjoint_insert_r_2. }
   { iApply (big_sepM2_insert_2 with "[Hx] HΔ"); simpl; eauto. }
   rewrite insert_commute//.
+  rewrite -insert_union_r //.
 Qed.
 
-Lemma tlolli_left (Δ Δ' : tyctx) τ1 τ2 e1 e2 σ (x y z : string) :
+Lemma tlolli_left (Γ Δ Δ' : tyctx) τ1 τ2 e1 e2 σ (x y z : string) :
   x ≠ y →
   x ≠ z →
   y ≠ z →
+  Γ !! x = None →
+  Γ !! y = None →
+  Γ !! z = None →
   Δ !! x = None →
   Δ' !! x = None →
   Δ !! y = None →
@@ -289,18 +557,18 @@ Lemma tlolli_left (Δ Δ' : tyctx) τ1 τ2 e1 e2 σ (x y z : string) :
   Δ !! z = None →
   Δ' !! z = None →
   Δ ##ₘ Δ' →
-  is_closed_expr_set ({[y]} ∪ dom stringset Δ') e1 →
-  is_closed_expr_set ({[x;z]} ∪ dom stringset Δ) e2 →
-  (Δ' ⊢ₗ e1 : (y : τ1)) -∗
-  (<[x:=τ2]>Δ ⊢ₗ e2 : (z : σ)) -∗
-  ((<[x:=τ1 ⊸ τ2]>Δ) ∪ Δ' ⊢ₗ (let: y := start_chan (λ: y, e1) in send x y;; e2) : (z : σ)).
+  is_closed_expr_set ({[y]} ∪ dom stringset Δ' ∪ dom stringset Γ) e1 →
+  is_closed_expr_set ({[x;z]} ∪ dom stringset Δ ∪ dom stringset Γ) e2 →
+  (Γ &; Δ' ⊢ₗ e1 : (y : τ1)) -∗
+  (Γ &; <[x:=τ2]>Δ ⊢ₗ e2 : (z : σ)) -∗
+  (Γ &; (<[x:=τ1 ⊸ τ2]>Δ) ∪ Δ' ⊢ₗ (let: y := start_chan (λ: y, e1) in send x y;; e2) : (z : σ)).
 Proof.
-  intros Hxy Hxz Hyz Hx Hx' Hy Hy' Hz Hz' HΔ He1 He2. iIntros "H1 H2".
-  iIntros (cs o) "Hcs Ho". simpl.
+  intros Hxy Hxz Hyz HxΓ HyΓ HzΓ Hx Hx' Hy Hy' Hz Hz' HΔ He1 He2.
+  iIntros "#H1 #H2". iModIntro.
+  iIntros (ss cs o Hsscs) "#Hss Hcs Ho". simpl.
   rewrite lookup_delete.
   rewrite !lookup_delete_ne//.
   rewrite lookup_insert_ne//.
-
   rewrite big_sepM2_union_l //; last first.
   { by eapply map_disjoint_insert_l_2. }
   iDestruct "Hcs" as (cs1 cs2 Hcs' ->) "[HΔ HΔ']".
@@ -309,33 +577,45 @@ Proof.
     iPureIntro. revert Hfoo. rewrite dom_insert_L. done. }
   iAssert (⌜dom stringset Δ' = dom stringset cs2⌝)%I as %Hdom2.
   { by rewrite (big_sepM2_dom _ _ cs2). }
+  iAssert (⌜dom stringset Γ = dom stringset ss⌝)%I as %Hdom0.
+  { by rewrite (big_sepM2_dom _ Γ). }
 
 
   assert_in_map cs1 x.
 
   assert_not_in_map cs1 y.
   assert_not_in_map cs2 y.
+  assert_not_in_map ss x.
+  assert_not_in_map ss y.
+
+  eapply map_disjoint_union_r in Hsscs.
+  destruct Hsscs as [Hsscs1 Hsscs2].
 
   wp_smart_apply (start_chan_spec (iProto_dual (interp_ty τ1)) with "[H1 HΔ']").
   { iNext. iIntros (c) "Hc".
     rewrite iProto_dual_involutive. wp_pures.
-    iSpecialize ("H1" with "HΔ' Hc").
+    iSpecialize ("H1" $! ss cs2 with "[%] Hss HΔ' Hc"); eauto.
     rewrite -subst_map_insert.
-    cut (subst_map (<[y:=c]> cs2) e1
-         = subst_map (<[y:=c]> (<[z:=o]> (cs1 ∪ cs2))) e1); first intros ->.
+    cut (subst_map (<[y:=c]> (ss ∪ cs2)) e1
+         = subst_map (<[y:=c]> (<[z:=o]> (ss ∪ (cs1 ∪ cs2)))) e1); first intros ->.
     { iApply (wp_wand with "H1"); eauto. }
-    eapply subst_map_fact_1; eauto.
-    - by rewrite -Hdom2.
+    rewrite assoc_L (map_union_comm ss cs1)// -assoc_L.
+    eapply (subst_map_fact_1); eauto.
+    - by rewrite (map_union_comm ss cs2) // dom_union_L -Hdom2 -Hdom0 assoc_L.
     - eapply not_elem_of_dom. rewrite -Hdom1.
       eapply not_elem_of_dom in Hz.
       set_solver.
-    - eapply not_elem_of_dom. rewrite -Hdom2.
-      by eapply not_elem_of_dom. }
+    - eapply not_elem_of_dom. rewrite dom_union_L -Hdom2 -Hdom0.
+      eapply not_elem_of_union; split; by eapply not_elem_of_dom.
+    - eapply map_disjoint_union_r; eauto.
+  }
 
   iIntros (yc) "Hy". wp_pures.
   case_decide; last naive_solver.
+  rewrite lookup_union_r //.
   rewrite (lookup_union_Some_l _ _ x y0) //.
-  rewrite big_sepM2_insert_acc //; last first.
+
+  rewrite (big_sepM2_insert_acc _ _ cs1 x) //; last first.
   { eapply lookup_insert. }
   iDestruct "HΔ" as "[Hx Hcs]".
   simpl.
@@ -343,204 +623,254 @@ Proof.
   wp_send with "[$Hy]". wp_pures.
   iSpecialize ("Hcs" with "Hx").
   rewrite insert_insert (insert_id cs1)//.
-  iSpecialize ("H2" with "Hcs Ho").
+  iSpecialize ("H2" $! ss _ with "[%] Hss Hcs Ho"); eauto.
   rewrite -subst_map_insert. rewrite insert_commute//.
-  cut (subst_map (<[z:=o]> cs1) e2
-       = subst_map (<[z:=o]> (<[y:=yc]> (cs1 ∪ cs2))) e2); first by intros ->.
+  cut (subst_map (<[z:=o]> (ss ∪ cs1)) e2
+       = subst_map (<[z:=o]> (<[y:=yc]> (ss ∪ (cs1 ∪ cs2)))) e2); first by intros ->.
+  rewrite assoc_L. rewrite (map_union_comm ss cs1)//.
   eapply subst_map_fact_0; eauto.
-  rewrite -Hdom1. rewrite union_assoc_L. by rewrite (union_comm_L {[z]}).
+  - rewrite dom_union_L -Hdom0 -Hdom1.
+    cut (({[z]} ∪ ({[x]} ∪ dom stringset Δ ∪ dom stringset Γ)) =
+         ({[x; z]} ∪ dom stringset Δ ∪ dom stringset Γ)) ; first by intros ->.
+    set_unfold. tauto.
+  - eapply lookup_union_None. tauto.
 Qed.
 
 
-Lemma twith_right Δ τ1 τ2 e1 e2 (x : string) :
-  Δ !! x = None →
-  (Δ ⊢ₗ e1 : (x : τ1)) -∗
-  (Δ ⊢ₗ e2 : (x : τ2)) -∗
-  Δ ⊢ₗ (if: recv x then e1 else e2) : (x : τ1 & τ2).
+Lemma twith_right Γ Δ τ1 τ2 e1 e2 (x : string) :
+  (Γ &; Δ ⊢ₗ e1 : (x : τ1)) -∗
+  (Γ &; Δ ⊢ₗ e2 : (x : τ2)) -∗
+  Γ &; Δ ⊢ₗ (if: recv x then e1 else e2) : (x : τ1 & τ2).
 Proof.
-  intros Hx. iIntros "H1 H2". iIntros (cs ox) "Hcs Hx /=".
+  iIntros "#H1 #H2". iModIntro.
+  iIntros (ss cs ox Hsscs) "Hss Hcs Hx /=".
   rewrite lookup_insert.
   wp_branch; wp_pures.
-  - iApply ("H1" with "Hcs Hx").
-  - iApply ("H2" with "Hcs Hx").
+  - iApply ("H1" $! ss cs with "[%] Hss Hcs Hx"); eauto.
+  - iApply ("H2" $! ss cs with "[%] Hss Hcs Hx"); eauto.
 Qed.
 
-Lemma twith_left_1 Δ τ1 τ2 e (x y : string) σ :
+Lemma twith_left_1 Γ Δ τ1 τ2 e (x y : string) σ :
   x ≠ y →
+  Γ !! x = None →
   Δ !! x = None →
-  (<[x:=τ1]>Δ ⊢ₗ e : (y : σ)) -∗
-  <[x:=τ1 & τ2]>Δ ⊢ₗ (send x #true;; e) : (y : σ).
+  (Γ &; <[x:=τ1]>Δ ⊢ₗ e : (y : σ)) -∗
+  Γ &; <[x:=τ1 & τ2]>Δ ⊢ₗ (send x #true;; e) : (y : σ).
 Proof.
-  intros Hxy HΔ. iIntros "H".
-  iIntros (cs oy) "Hcs Hy /=".
+  intros Hxy HΓ HΔ. iIntros "#H".
+  iModIntro. iIntros (ss cs oy Hsscs) "Hss Hcs Hy /=".
   iAssert (⌜{[x]} ∪ dom stringset Δ = dom stringset cs⌝)%I as %Hdom.
-  { by rewrite big_sepM2_dom dom_insert_L. }
+  { by rewrite (big_sepM2_dom _ _ cs) dom_insert_L. }
+  iAssert (⌜dom stringset Γ = dom stringset ss⌝)%I as %Hdom0.
+  { by rewrite (big_sepM2_dom _ _ ss). }
+
+
   assert_in_map_ cs x xv Hxv.
-  rewrite lookup_insert_ne// Hxv.
-  rewrite big_sepM2_insert_acc; eauto; last first.
+  assert_not_in_map ss x.
+
+  rewrite lookup_insert_ne//. rewrite lookup_union_r // Hxv.
+  rewrite (big_sepM2_insert_acc _ _ cs); eauto; last first.
   { eapply lookup_insert. }
   iDestruct "Hcs" as "[Hx Hcs]". iSimpl in "Hx".
   wp_select. wp_pures.
   iSpecialize ("Hcs" with "Hx").
   rewrite insert_insert // (insert_id cs)//.
-  iApply ("H"  with "Hcs Hy").
+  by iApply ("H"  with "[%] Hss Hcs Hy").
 Qed.
 
-Lemma twith_left_2 Δ τ1 τ2 e (x y : string) σ :
+Lemma twith_left_2 Γ Δ τ1 τ2 e (x y : string) σ :
   x ≠ y →
+  Γ !! x = None →
   Δ !! x = None →
-  (<[x:=τ2]>Δ ⊢ₗ e : (y : σ)) -∗
-  <[x:=τ1 & τ2]>Δ ⊢ₗ (send x #false;; e) : (y : σ).
+  (Γ &; <[x:=τ2]>Δ ⊢ₗ e : (y : σ)) -∗
+  Γ &; <[x:=τ1 & τ2]>Δ ⊢ₗ (send x #false;; e) : (y : σ).
 Proof.
-  intros Hxy HΔ. iIntros "H".
-  iIntros (cs oy) "Hcs Hy /=".
+  intros Hxy HΓ HΔ. iIntros "#H".
+  iModIntro. iIntros (ss cs oy Hsscs) "Hss Hcs Hy /=".
   iAssert (⌜{[x]} ∪ dom stringset Δ = dom stringset cs⌝)%I as %Hdom.
-  { by rewrite big_sepM2_dom dom_insert_L. }
+  { by rewrite (big_sepM2_dom _ _ cs) dom_insert_L. }
+  iAssert (⌜dom stringset Γ = dom stringset ss⌝)%I as %Hdom0.
+  { by rewrite (big_sepM2_dom _ _ ss). }
+
+
   assert_in_map_ cs x xv Hxv.
-  rewrite lookup_insert_ne// Hxv.
-  rewrite big_sepM2_insert_acc; eauto; last first.
+  assert_not_in_map ss x.
+
+  rewrite lookup_insert_ne//. rewrite lookup_union_r // Hxv.
+  rewrite (big_sepM2_insert_acc _ _ cs); eauto; last first.
   { eapply lookup_insert. }
   iDestruct "Hcs" as "[Hx Hcs]". iSimpl in "Hx".
   wp_select. wp_pures.
   iSpecialize ("Hcs" with "Hx").
   rewrite insert_insert // (insert_id cs)//.
-  iApply ("H"  with "Hcs Hy").
+  by iApply ("H"  with "[%] Hss Hcs Hy").
 Qed.
 
-Lemma tplus_right_1 Δ τ1 τ2 e (x : string) :
-  Δ !! x = None →
-  (Δ ⊢ₗ e : (x : τ1)) -∗
-  Δ ⊢ₗ (send x #true;; e) : (x : τ1 ⊕ τ2).
+Lemma tplus_right_1 Γ Δ τ1 τ2 e (x : string) :
+  (Γ &; Δ ⊢ₗ e : (x : τ1)) -∗
+  Γ &; Δ ⊢ₗ (send x #true;; e) : (x : τ1 ⊕ τ2).
 Proof.
-  intros Hx. iIntros "H1". iIntros (cs ox) "Hcs Hx /=".
+  iIntros "#H1". iModIntro.
+  iIntros (ss cs ox Hsscs) "Hss Hcs Hx /=".
   rewrite lookup_insert.
   wp_select. wp_pures.
-  iApply ("H1" with "Hcs Hx").
+  iApply ("H1" with "[%//] Hss Hcs Hx").
 Qed.
 
-Lemma tplus_right_2 Δ τ1 τ2 e (x : string) :
-  Δ !! x = None →
-  (Δ ⊢ₗ e : (x : τ2)) -∗
-  Δ ⊢ₗ (send x #false;; e) : (x : τ1 ⊕ τ2).
+Lemma tplus_right_2 Γ Δ τ1 τ2 e (x : string) :
+  (Γ &; Δ ⊢ₗ e : (x : τ2)) -∗
+  Γ &; Δ ⊢ₗ (send x #false;; e) : (x : τ1 ⊕ τ2).
 Proof.
-  intros Hx. iIntros "H1". iIntros (cs ox) "Hcs Hx /=".
+  iIntros "#H1". iModIntro.
+  iIntros (ss cs ox Hsscs) "Hss Hcs Hx /=".
   rewrite lookup_insert.
   wp_select. wp_pures.
-  iApply ("H1" with "Hcs Hx").
+  iApply ("H1" with "[%//] Hss Hcs Hx").
 Qed.
 
-Lemma tplus_left Δ τ1 τ2 e1 e2 (x y : string) σ :
+Lemma tplus_left Γ Δ τ1 τ2 e1 e2 (x y : string) σ :
   x ≠ y →
+  Γ !! x = None →
   Δ !! x = None →
-  (<[x:=τ1]>Δ ⊢ₗ e1 : (y : σ)) -∗
-  (<[x:=τ2]>Δ ⊢ₗ e2 : (y : σ)) -∗
-  <[x:=τ1⊕τ2]>Δ ⊢ₗ (if: recv x then e1 else e2) : (y : σ).
+  (Γ &; <[x:=τ1]>Δ ⊢ₗ e1 : (y : σ)) -∗
+  (Γ &; <[x:=τ2]>Δ ⊢ₗ e2 : (y : σ)) -∗
+  Γ &; <[x:=τ1⊕τ2]>Δ ⊢ₗ (if: recv x then e1 else e2) : (y : σ).
 Proof.
-  intros Hxy HΔ. iIntros "He1 He2".
-  iIntros (cs oy) "Hcs Hy /=".
+  intros Hxy HΓ HΔ. iIntros "#He1 #He2". iModIntro.
+  iIntros (ss cs oy Hsscs) "Hss Hcs Hy /=".
   iAssert (⌜{[x]} ∪ dom stringset Δ = dom stringset cs⌝)%I as %Hdom.
-  { by rewrite big_sepM2_dom dom_insert_L. }
+  { by rewrite (big_sepM2_dom _ _ cs) dom_insert_L. }
+  iAssert (⌜dom stringset Γ = dom stringset ss⌝)%I as %Hdom0.
+  { by rewrite (big_sepM2_dom _ _ ss). }
   assert_in_map_ cs x xv Hxv.
-  rewrite lookup_insert_ne// Hxv.
-  rewrite big_sepM2_insert_acc; eauto; last first.
+  assert_not_in_map ss x.
+  rewrite lookup_insert_ne// lookup_union_r // Hxv.
+  rewrite (big_sepM2_insert_acc _ _ cs); eauto; last first.
   { eapply lookup_insert. }
   iDestruct "Hcs" as "[Hx Hcs]". iSimpl in "Hx".
   wp_branch; wp_pures.
   - iSpecialize ("Hcs" with "Hx").
     rewrite insert_insert (insert_id cs) //.
-    iApply ("He1" with "Hcs Hy").
+    iApply ("He1" with "[%//] Hss Hcs Hy").
   - iSpecialize ("Hcs" with "Hx").
     rewrite insert_insert (insert_id cs) //.
-    iApply ("He2" with "Hcs Hy").
+    iApply ("He2" with "[%//] Hss Hcs Hy").
 Qed.
 
-Lemma ttimes_right (Δ Δ' : tyctx) τ1 τ2 e e' (x y : string) :
+Lemma ttimes_right (Γ Δ Δ' : tyctx) τ1 τ2 e e' (x y : string) :
   x ≠ y →
   Δ ##ₘ Δ' →
+  Γ !! x = None →
+  Γ !! y = None →
   Δ !! y = None →
   Δ' !! y = None →
   Δ !! x = None →
   Δ' !! x = None →
-  is_closed_expr_set ({[x]} ∪ dom stringset Δ) e →
-  is_closed_expr_set ({[y]} ∪ dom stringset Δ') e' →
-  (Δ ⊢ₗ e : (x : τ1)) -∗
-  (Δ' ⊢ₗ e' : (y : τ2)) -∗
-  (Δ ∪ Δ' ⊢ₗ (let: x := start_chan (λ: x, e) in
-              send y x;;
-              e') : (y : τ1 ⊗ τ2)).
+  is_closed_expr_set ({[x]} ∪ dom stringset Δ ∪ dom stringset Γ) e →
+  is_closed_expr_set ({[y]} ∪ dom stringset Δ' ∪ dom stringset Γ) e' →
+  (Γ &; Δ ⊢ₗ e : (x : τ1)) -∗
+  (Γ &; Δ' ⊢ₗ e' : (y : τ2)) -∗
+  (Γ &; Δ ∪ Δ' ⊢ₗ (let: x := start_chan (λ: x, e) in
+                   send y x;;
+                   e') : (y : τ1 ⊗ τ2)).
 Proof.
-  intros Hxy HΔ Hy1 Hy2 Hx1 Hx2 Hcle Hcle'. iIntros "H1 H2".
-  iIntros (cs oy) "HΔ Hoy". wp_pures.
+  intros Hxy HΔ Hx0 Hy0 Hy1 Hy2 Hx1 Hx2 Hcle Hcle'. iIntros "#H1 #H2". iModIntro.
+  iIntros (ss cs oy Hsscs) "#Hss HΔ Hoy". wp_pures.
   rewrite lookup_delete_ne// !lookup_delete lookup_insert.
   simpl.
   rewrite big_sepM2_union_l //.
   iDestruct "HΔ" as (cs1 cs2 Hcs ->) "[HΔ HΔ']".
 
   iAssert (⌜dom stringset Δ = dom stringset cs1⌝)%I as %Hdom1.
-  { by rewrite big_sepM2_dom. }
+  { by rewrite (big_sepM2_dom _ Δ). }
   iAssert (⌜dom stringset Δ' = dom stringset cs2⌝)%I as %Hdom2.
   { by rewrite (big_sepM2_dom _ Δ'). }
+  iAssert (⌜dom stringset Γ = dom stringset ss⌝)%I as %Hdom0.
+  { by rewrite (big_sepM2_dom _ Γ). }
   assert_not_in_map cs1 y.
   assert_not_in_map cs2 y.
   assert_not_in_map cs1 x.
   assert_not_in_map cs2 x.
+  assert_not_in_map ss x.
+  assert_not_in_map ss y.
 
+  eapply map_disjoint_union_r in Hsscs. destruct Hsscs as [Hsscs1 Hsscs2].
   wp_smart_apply (start_chan_spec (iProto_dual (interp_ty τ1)) with "[H1 HΔ]").
   { iNext. iIntros (c) "Hc".
     rewrite iProto_dual_involutive. wp_pures.
-    iSpecialize ("H1" with "HΔ Hc").
+    iSpecialize ("H1" with "[%] Hss HΔ Hc"); eauto.
     rewrite -subst_map_insert.
-    assert (subst_map (<[x:=c]> cs1) e
-         = subst_map (<[x:=c]> (<[y:=oy]> (cs1 ∪ cs2))) e) as ->.
-    { eapply subst_map_fact_0; eauto.
-      by rewrite -Hdom1. }
+    assert (subst_map (<[x:=c]> (ss ∪ cs1)) e
+         = subst_map (<[x:=c]> (<[y:=oy]> (ss ∪ (cs1 ∪ cs2)))) e) as ->.
+    { rewrite assoc_L.
+      eapply subst_map_fact_0; eauto.
+      - rewrite dom_union_L -Hdom1 -Hdom0.
+        assert (({[x]} ∪ (dom stringset Γ ∪ dom stringset Δ)) =
+                ({[x]} ∪ dom stringset Δ ∪ dom stringset Γ)) as ->.
+        { set_unfold; tauto. }
+        done.
+      - eapply lookup_union_None. tauto.
+    }
     iApply (wp_wand with "H1"); eauto. }
   iIntros (xc) "Hxc". wp_pures.
   case_decide; last naive_solver.
   wp_send with "[$Hxc]". wp_pures.
-  iSpecialize ("H2" with "HΔ' Hoy").
+  iSpecialize ("H2" with "[%] Hss HΔ' Hoy"); eauto.
   rewrite -subst_map_insert. rewrite insert_commute //.
-  rewrite -(subst_map_fact_1 cs1 cs2 y x)//.
-  by rewrite -Hdom2.
+  rewrite assoc_L (map_union_comm ss cs1) //.
+  rewrite -assoc_L.
+  rewrite -(subst_map_fact_1 cs1 (ss ∪ cs2) y x)//.
+  - rewrite dom_union_L -Hdom0 -Hdom2.
+    cut (({[y]} ∪ (dom stringset Γ ∪ dom stringset Δ')) =
+         ({[y]} ∪ dom stringset Δ' ∪ dom stringset Γ)); first by intros ->.
+    set_unfold. tauto.
+  - eapply lookup_union_None. tauto.
+  - eapply map_disjoint_union_r. eauto.
 Qed.
 
-Lemma ttimes_left (Δ : tyctx) τ1 τ2 (x y : string) (c : string) σ e :
+Lemma ttimes_left (Γ Δ : tyctx) τ1 τ2 (x y : string) (c : string) σ e :
   x ≠ y →
   x ≠ c →
   y ≠ c →
+  Γ !! x = None →
+  Γ !! y = None →
   Δ !! x = None →
   Δ !! y = None →
-  ((<[y:=τ1]>(<[x:=τ2]>Δ)) ⊢ₗ e : (c : σ)) -∗
-  ((<[x:=τ1 ⊗ τ2]>Δ) ⊢ₗ (let: y := recv x in e) : (c : σ)).
+  (Γ &; (<[y:=τ1]>(<[x:=τ2]>Δ)) ⊢ₗ e : (c : σ)) -∗
+  (Γ &; (<[x:=τ1 ⊗ τ2]>Δ) ⊢ₗ (let: y := recv x in e) : (c : σ)).
 Proof.
-  intros Hxy Hxc Hyc Hx Hy. iIntros "IH".
-  iIntros (cs o) "Hcs Ho". simpl.
+  intros Hxy Hxc Hyc Hx0 Hy0 Hx Hy. iIntros "#IH". iModIntro.
+  iIntros (ss cs o Hsscs) "Hss Hcs Ho". simpl.
   rewrite lookup_insert_ne//.
 
   iAssert (⌜{[x]} ∪ dom stringset Δ = dom stringset cs⌝)%I as %Hdom.
   { by rewrite (big_sepM2_dom _ _ cs) dom_insert_L. }
+  iAssert (⌜dom stringset Γ = dom stringset ss⌝)%I as %Hdom0.
+  { by rewrite (big_sepM2_dom _ _ ss). }
 
-  assert_in_map_ cs x cx Hcx. rewrite Hcx.
+  assert_in_map_ cs x cx Hcx.
   assert_not_in_map cs y.
-  rewrite big_sepM2_insert_acc; eauto; last first.
+  assert_not_in_map ss x.
+  assert_not_in_map ss y.
+  rewrite lookup_union_r // Hcx.
+
+  rewrite (big_sepM2_insert_acc _ _ cs); eauto; last first.
   { eapply lookup_insert. }
   iDestruct "Hcs" as "[Hx Hcs]". iSimpl in "Hx".
   wp_recv (cy) as "Hy". wp_pures.
   rewrite -subst_map_insert.
   iSpecialize ("Hcs" with "Hx").
   rewrite insert_insert (insert_id cs) //.
-  iSpecialize ("IH" $! (<[y:=cy]>(map_insert x cx cs)) with "[Hcs Hy] Ho").
+  iSpecialize ("IH" $! ss (<[y:=cy]>(<[x:=cx]> cs)) with "[%] Hss [Hcs Hy] Ho").
+  { eapply map_disjoint_insert_r; split; eauto.
+    eapply map_disjoint_insert_r. split; eauto. }
   { iApply big_sepM2_insert.
     - rewrite lookup_insert_ne//.
-    - replace (map_insert x cx cs) with (<[x:=cx]>cs) by reflexivity.
-      rewrite lookup_insert_ne//.
+    - rewrite lookup_insert_ne//.
     - iFrame "Hy".
-      replace (map_insert x cx cs) with (<[x:=cx]>cs) by reflexivity.
       rewrite (insert_id cs)//. }
-  replace (map_insert x cx cs) with (<[x:=cx]>cs) by reflexivity.
   rewrite (insert_id cs)//.
   rewrite insert_commute//.
+  rewrite -insert_union_r//.
 Qed.
 
-Lemma tofc_right Δ τ1 τ2 (x y : string) σ e :
-  
